viper-total-heaps/TotalFraming.thy
@@ -103,4 +103,12 @@ lemma pred_self_framing_subst:
   by blast
 
 
+subsection \<open>Context All Predicates Self-Framing\<close>
+
+definition ctxt_pred_self_framing :: "'a total_context \<Rightarrow> bool" where
+  "ctxt_pred_self_framing ctxt \<equiv> \<forall>pid pdecl.
+     ViperLang.predicates (program_total ctxt) pid = Some pdecl \<longrightarrow>
+     pred_self_framing ctxt pdecl"
+
+
 end
