viper-total-heaps/InhaleRel.thy
@@ -605,10 +605,10 @@ next
   thus "StateCons \<omega>' \<and>
         consistent_external (total_context.make Pr (\<lambda>_. None) (\<lambda>_. undefined)) (get_total_full \<omega>')"
     apply (intro conjI)
-    apply (unfold inhale_acc_normal_premise_def inhale_perm_single_def)[1]
+     apply (unfold inhale_acc_normal_premise_def inhale_perm_single_def)[1]
     using state_rel_consistent[OF StateRel[OF \<open>R \<omega> ns\<close>]]
      apply auto[1]
-    by (metis \<open>consistent_state_rel_opt (state_rel_opt Tr) \<Longrightarrow> StateCons \<omega> \<and> StateCons \<omega> \<and> consistent_external (total_context.make Pr (\<lambda>_. None) (\<lambda>_. undefined)) (get_total_full \<omega>) \<and> consistent_external (total_context.make Pr (\<lambda>_. None) (\<lambda>_. undefined)) (get_total_full \<omega>)\<close> extcons_preserved_by_inhale_acc inhale_acc_normal_premise_def ref.distinct(1))
+    by (metis state_rel_consistent[OF StateRel[OF \<open>R \<omega> ns\<close>]] extcons_preserved_by_inhale_perm_single inhale_acc_normal_premise_def ref.simps(3))
 qed
 
 subsection \<open>Pure expression rule\<close>
