viper-total-heaps/TotalConsistencyInst.thy
@@ -1,5 +1,5 @@
 theory TotalConsistencyInst
-  imports TotalSemantics TotalIntConsPreservation
+  imports TotalSemantics TotalIntConsPreservation TotalExtConsPreservation
 begin
 
 
@@ -8,12 +8,14 @@ subsection \<open>Internal Consistency Wellfoundness\<close>
 lemma wf_total_consistency_internal: "wf_total_consistency ctxt consistent_internal_total_full consistent_internal_total"
   unfolding wf_total_consistency_def
   apply (intro conjI)
-      apply (rule intcons_mono_prop_downward)
-     apply (simp add: intcons_empty is_empty_total_full_def)
+       apply (rule intcons_mono_prop_downward)
+      apply (simp add: intcons_empty is_empty_total_full_def)
   using intcons_preserved_by_red_stmt
-    apply blast
-   apply (simp add: intcons_preserved_by_update_store)
+     apply blast
+    apply (simp add: intcons_preserved_by_update_store)
   using consistent_internal_total_full_def
+   apply blast
+  using extcons_preserved_by_red_stmt
   by blast
 
 
